Drop label if no goto in body.

pulse/src/checker/Pulse.Checker.ForwardJumpLabel.fst
@@ -24,7 +24,9 @@ open Pulse.Typing
 open Pulse.Checker.Pure
 open Pulse.Checker.Base
 open Pulse.Checker.Prover
+module RU = Pulse.RuntimeUtils
 
+#push-options "--z3rlimit 10 --split_queries always"
 let check
     (g:env)
     (pre:term)
@@ -47,32 +49,52 @@ let check
       | PostHint ph ->
         ph
   in
+  if not (EffectAnnotSTT? post.effect_annot) then
+    fail g (Some rng) "Labels require stt" else
   let lbl_c = C_ST {
     u = post.u;
     res = post.ret_ty;
     pre = post.post;
-    post = tm_pure tm_false;
+    post = tm_pure tm_l_false;
   } in
   let lbl_x = fresh g in
   let g' = push_goto g lbl_x lbl lbl_c in
-  let pre_typing': tot_typing g' pre tm_slprop = admit () in
-  let post_hint' : post_hint_opt g' = admit (); PostHint post in
+  let pre_typing': tot_typing g' pre tm_slprop = RU.magic () in
+  let post_hint' : post_hint_opt g' =
+    assume post_hint_for_env_p g' post;
+    PostHint post in
   let body = open_st_term_nv body (lbl, lbl_x) in
   let body' = check g' pre pre_typing' post_hint' res_ppname body in
-  let (| body', body'_c, body'_typing |) = apply_checker_result_k #g #pre #post body' res_ppname in
+  let (| body', body'_c, body'_typing |) = apply_checker_result_k #g' #pre #post body' res_ppname in
   assert comp_u body'_c == comp_u lbl_c;
   assert comp_res body'_c == comp_res lbl_c;
   assert comp_pre body'_c == pre;
   assert comp_post body'_c == post.post;
-  let t = wtag (Some STT) (Tm_ForwardJumpLabel {
-    lbl = lbl;
-    body = close_st_term body' lbl_x;
-    post = body'_c;
-  }) in
-  let typing: st_typing g t body'_c =
-    T_ForwardJumpLabel g (lbl, lbl_x) body' _ body'_typing in
-  let (| c'', typing'' |) = match_comp_res_with_post_hint typing post_hint0 in
-  prove_post_hint #g
-    (try_frame_pre false #g pre_typing (|_,c'',typing''|) res_ppname)
-    post_hint0
-    rng
+  assert C_ST? body'_c;
+  assert lbl_c == goto_comp_of_block_comp body'_c;
+  let body = close_st_term body' lbl_x in
+  if not (lbl_x `Set.mem` freevars_st body) then (
+    // drop label if no goto in body
+    assume body == body';
+    let body_typing: st_typing g body' body'_c = RU.magic () in
+    let (| c'', typing'' |) = match_comp_res_with_post_hint body_typing post_hint0 in
+    prove_post_hint #g
+      (try_frame_pre false #g pre_typing (|_,c'',typing''|) res_ppname)
+      post_hint0
+      rng
+  ) else (
+    let t = wtag (Some STT) (Tm_ForwardJumpLabel {
+      lbl = lbl;
+      body = close_st_term body' lbl_x;
+      post = body'_c;
+    }) in
+    assume open_st_term' body (term_of_nvar (lbl, lbl_x)) 0 == body';
+    let typing: st_typing g t body'_c =
+      T_ForwardJumpLabel g (lbl, lbl_x) body body'_c body'_typing in
+    let (| c'', typing'' |) = match_comp_res_with_post_hint typing post_hint0 in
+    prove_post_hint #g
+      (try_frame_pre false #g pre_typing (|_,c'',typing''|) res_ppname)
+      post_hint0
+      rng
+  )
+#pop-options
